coq_general_theory/formula.v
@@ -1,0 +1,12 @@
+Require Import Floats.
+Require Import Strings.String.
+Open Scope string_scope.
+
+Inductive RatExpr : Type :=
+  | Const:  float -> RatExpr
+  | OneVar: string -> RatExpr
+  | Sum:    RatExpr -> RatExpr -> RatExpr
+  | Sub:    RatExpr -> RatExpr -> RatExpr
+  | Mul:    RatExpr -> RatExpr -> RatExpr
+  | Div:    RatExpr -> RatExpr -> RatExpr
+  | Minus:  RatExpr -> RatExpr.
